src/prop/Cover.v
@@ -1,0 +1,75 @@
+From sflib Require Import sflib.
+From Paco Require Import paco.
+
+From PromisingLib Require Import Axioms.
+From PromisingLib Require Import Basic.
+From PromisingLib Require Import DataStructure.
+From PromisingLib Require Import DenseOrder.
+From PromisingLib Require Import Loc.
+From PromisingLib Require Import Language.
+From PromisingLib Require Import Event.
+
+Require Import Time.
+Require Import View.
+Require Import Cell.
+Require Import Memory.
+
+Set Implicit Arguments.
+
+
+Variant covered (loc:Loc.t) (ts:Time.t) (mem:Memory.t): Prop :=
+| covered_intro
+    from to msg
+    (GET: Memory.get loc to mem = Some (from, msg))
+    (ITV: Interval.mem (from, to) ts)
+.
+
+Lemma covered_disjoint
+      mem1 mem2 loc from to
+      (COVER: forall loc ts, covered loc ts mem1 -> covered loc ts mem2)
+      (DISJOINT: forall to2 from2 msg2
+                   (GET2: Memory.get loc to2 mem2 = Some (from2, msg2)),
+          Interval.disjoint (from, to) (from2, to2)):
+  forall to2 from2 msg2
+    (GET2: Memory.get loc to2 mem1 = Some (from2, msg2)),
+    Interval.disjoint (from, to) (from2, to2).
+Proof.
+  ii. exploit COVER; eauto.
+  { econs; eauto. }
+  intros x0. inv x0. eapply DISJOINT; eauto.
+Qed.
+
+Lemma get_disjoint_covered_disjoint
+      mem loc from to:
+  (forall t f m, Memory.get loc t mem = Some (f, m) -> Interval.disjoint (from, to) (f, t)) ->
+  (forall ts, covered loc ts mem -> ~ Interval.mem (from, to) ts).
+Proof.
+  ii. inv H0. eapply H; eauto.
+Qed.
+
+Lemma covered_disjoint_get_disjoint
+      mem loc from to:
+  (forall ts, covered loc ts mem -> ~ Interval.mem (from, to) ts) ->
+  (forall t f m, Memory.get loc t mem = Some (f, m) -> Interval.disjoint (from, to) (f, t)).
+Proof.
+  ii. eapply H; eauto. econs; eauto.
+Qed.
+
+Lemma add_covered
+      mem2 mem1 loc from to msg
+      l t
+      (ADD: Memory.add mem1 loc from to msg mem2):
+  covered l t mem2 <->
+  covered l t mem1 \/ (l = loc /\ Interval.mem (from, to) t).
+Proof.
+  econs; i.
+  - inv H. revert GET. erewrite Memory.add_o; eauto. condtac; ss.
+    + des. subst. i. inv GET. auto.
+    + left. econs; eauto.
+  - des.
+    + inv H. econs; eauto.
+      erewrite Memory.add_o; eauto. condtac; ss; eauto.
+      des. subst. exploit Memory.add_get0; eauto. i. des. congr.
+    + subst. econs; eauto. erewrite Memory.add_o; eauto. condtac; ss.
+      des; congr.
+Qed.
