src/trans/SimMemory.v
@@ -1,0 +1,210 @@
+Require Import RelationClasses.
+
+From sflib Require Import sflib.
+From Paco Require Import paco.
+
+From PromisingLib Require Import Axioms.
+From PromisingLib Require Import Basic.
+From PromisingLib Require Import Loc.
+From PromisingLib Require Import DenseOrder.
+From PromisingLib Require Import Language.
+
+From PromisingLib Require Import Event.
+Require Import Time.
+Require Import View.
+Require Import Cell.
+Require Import Memory.
+Require Import TView.
+Require Import Local.
+Require Import Thread.
+Require Import Configuration.
+
+Require Import Cover.
+
+Set Implicit Arguments.
+
+
+Inductive sim_memory (mem_src mem_tgt:Memory.t): Prop :=
+| sim_memory_intro
+    (COVER: forall loc ts, covered loc ts mem_src <-> covered loc ts mem_tgt)
+    (MSG: forall loc from_tgt to msg_tgt
+            (GET: Memory.get loc to mem_tgt = Some (from_tgt, msg_tgt)),
+        exists from_src msg_src,
+          <<GET: Memory.get loc to mem_src = Some (from_src, msg_src)>> /\
+          <<MSG: Message.le msg_src msg_tgt>>)
+.
+
+Global Program Instance sim_memory_PreOrder: PreOrder sim_memory.
+Next Obligation.
+  econs; try refl. i. esplits; eauto. refl.
+Qed.
+Next Obligation.
+  ii. inv H. inv H0. econs; try etrans; eauto. i.
+  exploit MSG0; eauto. i. des.
+  exploit MSG; eauto. i. des.
+  esplits; eauto. etrans; eauto.
+Qed.
+
+
+Lemma sim_memory_get
+      loc from_tgt to msg_tgt mem_src mem_tgt
+      (SIM: sim_memory mem_src mem_tgt)
+      (GET: Memory.get loc to mem_tgt = Some (from_tgt, msg_tgt)):
+  exists from_src msg_src,
+    <<GET: Memory.get loc to mem_src = Some (from_src, msg_src)>> /\
+    <<MSG: Message.le msg_src msg_tgt>>.
+Proof.
+  eapply SIM. eauto.
+Qed.
+
+Lemma sim_memory_get_inv
+      loc from_src to_src msg_src mem_src
+      mem_tgt
+      (INHABITED_SRC: Memory.inhabited mem_src)
+      (INHABITED_TGT: Memory.inhabited mem_tgt)
+      (SIM: sim_memory mem_src mem_tgt)
+      (GET_SRC: Memory.get loc to_src mem_src = Some (from_src, msg_src)):
+  exists from_tgt to_tgt msg_tgt,
+    <<FROM: Time.le from_tgt from_src>> /\
+    <<TO: Time.le to_src to_tgt>> /\
+    <<GET_TGT: Memory.get loc to_tgt mem_tgt = Some (from_tgt, msg_tgt)>>.
+Proof.
+  destruct (Time.eq_dec to_src Time.bot).
+  { subst. rewrite INHABITED_SRC in GET_SRC. inv GET_SRC.
+    esplits; try refl. apply INHABITED_TGT.
+  }
+  dup SIM. inv SIM0. dup COVER. specialize (COVER0 loc to_src). des.
+  exploit COVER0.
+  { econs; eauto. econs; try refl.
+    exploit Memory.get_ts; eauto. i. des; subst; timetac.
+  }
+  intros x. dup x. inv x0. esplits; eauto.
+  - destruct (Time.le_lt_dec from from_src); ss.
+    dup COVER. specialize (COVER2 loc from). des. exploit COVER2.
+    { econs; eauto.
+      exploit Memory.get_ts; try exact GET_SRC. i. des; ss.
+      inv ITV. econs; eauto. econs. ss.
+    }
+    intros x0. inv x0.
+    destruct (Time.eq_dec to0 from).
+    + subst. exploit MSG; try exact GET0. i. des.
+      exploit Memory.get_disjoint; [exact GET_SRC|exact GET1|..]. i. des.
+      * subst. inv ITV. timetac.
+      * exfalso. apply (x1 from).
+        { inv ITV. econs; eauto. s. econs; eauto. }
+        { econs; try refl. s.
+          exploit Memory.get_ts; try exact GET1. i. des; ss.
+          subst. inv ITV0. inv FROM. }
+    + exploit Memory.get_disjoint; [exact GET|exact GET0|..]. i. des.
+      * subst. inv ITV0. timetac.
+      * exfalso. destruct (Time.le_lt_dec to to0).
+        { apply (x1 to).
+          - econs; try refl.
+            exploit Memory.get_ts; try exact GET. i. des; ss.
+            subst. inv ITV0. inv FROM.
+          - econs; eauto. inv ITV0. ss.
+            exploit Memory.get_ts; try exact GET. i. des; ss.
+            + subst. inv l.
+            + eapply TimeFacts.lt_le_lt; eauto. econs; eauto. }
+        { apply (x1 to0).
+          - inv ITV0. econs; ss.
+            + inv TO; ss. inv H. congr.
+            + econs. ss.
+          - econs; try refl.
+            exploit Memory.get_ts; try exact GET0. i. des; ss.
+            subst. inv ITV0. ss. inv TO; inv H. inv FROM. }
+  - inv ITV. ss.
+Qed.
+
+Lemma sim_memory_max_ts
+      mem_src mem_tgt loc
+      (SIM: sim_memory mem_src mem_tgt)
+      (CLOSED_SRC: Memory.closed mem_src)
+      (CLOSED_TGT: Memory.closed mem_tgt):
+  Memory.max_ts loc mem_src = Memory.max_ts loc mem_tgt.
+Proof.
+  inv SIM. inv CLOSED_SRC. inv CLOSED_TGT.
+  clear MSG CLOSED CLOSED0.
+  apply TimeFacts.antisym.
+  - specialize (COVER loc (Memory.max_ts loc mem_src)). des.
+    exploit Memory.max_ts_spec; try eapply (INHABITED loc). i. des.
+    exploit Memory.get_ts; eauto. i. des.
+    { rewrite x1. apply Time.bot_spec. }
+    exploit COVER.
+    { econs; eauto. econs; eauto. refl. }
+    intros x. inv x. exploit Memory.max_ts_spec; try exact GET0. i. des.
+    inv ITV. ss. etrans; eauto.
+  - specialize (COVER loc (Memory.max_ts loc mem_tgt)). des.
+    exploit Memory.max_ts_spec; try eapply (INHABITED0 loc). i. des.
+    exploit Memory.get_ts; eauto. i. des.
+    { rewrite x1. apply Time.bot_spec. }
+    exploit COVER0.
+    { econs; eauto. econs; eauto. refl. }
+    intros x. inv x. exploit Memory.max_ts_spec; try exact GET0. i. des.
+    inv ITV. ss. etrans; eauto.
+Qed.
+
+Lemma sim_memory_add
+      mem1_src mem1_tgt msg_src
+      mem2_src mem2_tgt msg_tgt
+      loc from to
+      (MSG: Message.le msg_src msg_tgt)
+      (SRC: Memory.add mem1_src loc from to msg_src mem2_src)
+      (TGT: Memory.add mem1_tgt loc from to msg_tgt mem2_tgt)
+      (SIM: sim_memory mem1_src mem1_tgt):
+  sim_memory mem2_src mem2_tgt.
+Proof.
+  inv SIM. econs; i.
+  - rewrite add_covered; [|eauto]. rewrite (@add_covered mem2_tgt); [|eauto].
+    econs; i; des; (try by right).
+    + left. eapply COVER. eauto.
+    + left. eapply COVER. eauto.
+  - revert GET. erewrite Memory.add_o; eauto. condtac; ss.
+    + des. subst. i. inv GET. esplits; eauto.
+      erewrite Memory.add_o; eauto. condtac; ss.
+    + erewrite (@Memory.add_o mem2_src); eauto. condtac; ss. eauto.
+Qed.
+
+Lemma sim_memory_closed_timemap
+      mem_src mem_tgt
+      tm
+      (SIM: sim_memory mem_src mem_tgt)
+      (TGT: Memory.closed_timemap tm mem_tgt):
+  Memory.closed_timemap tm mem_src.
+Proof.
+  ii. exploit TGT; eauto. i. des.
+  exploit sim_memory_get; eauto. i. des.
+  inv MSG. eauto.
+Qed.
+
+Lemma sim_memory_closed_view
+      mem_src mem_tgt
+      view
+      (SIM: sim_memory mem_src mem_tgt)
+      (TGT: Memory.closed_view view mem_tgt):
+  Memory.closed_view view mem_src.
+Proof.
+  econs.
+  - eapply sim_memory_closed_timemap; eauto. apply TGT.
+  - eapply sim_memory_closed_timemap; eauto. apply TGT.
+Qed.
+
+Lemma sim_memory_closed_opt_view
+      mem_src mem_tgt
+      view
+      (SIM: sim_memory mem_src mem_tgt)
+      (TGT: Memory.closed_opt_view view mem_tgt):
+  Memory.closed_opt_view view mem_src.
+Proof.
+  inv TGT; econs. eapply sim_memory_closed_view; eauto.
+Qed.
+
+Lemma sim_memory_closed_message
+      mem_src mem_tgt
+      msg
+      (SIM: sim_memory mem_src mem_tgt)
+      (TGT: Memory.closed_message msg mem_tgt):
+  Memory.closed_message msg mem_src.
+Proof.
+  inv TGT; ss. econs. eapply sim_memory_closed_opt_view; eauto.
+Qed.
